@prefix : <http://ethon.consensys.net/> .
@prefix dc: <http://purl.org/dc/elements/1.1/> .
@prefix ns: <http://www.w3.org/2003/06/sw-vocab-status/ns#> .
@prefix v0: <http://ethon.consensys.net/v0/> .
@prefix owl: <http://www.w3.org/2002/07/owl#> .
@prefix rdf: <http://www.w3.org/1999/02/22-rdf-syntax-ns#> .
@prefix xml: <http://www.w3.org/XML/1998/namespace> .
@prefix xsd: <http://www.w3.org/2001/XMLSchema#> .
@prefix rdfs: <http://www.w3.org/2000/01/rdf-schema#> .
@prefix vann: <http://purl.org/vocab/vann/> .

<http://ethon.consensys.net/> a owl:Ontology ;
	owl:versionIRI <http://ethon.consensys.net/v0/> ;
	owl:imports <http://www.w3.org/2003/06/sw-vocab-status/ns> ;
	rdfs:seeAlso <https://github.com/ethereum/yellowpaper> ;
	dc:contributor "Shahan Khatchadourian" , "Sunny Aggarwal" ;
	dc:creator "Johannes Pfeffer" ;
	ns:term_status "testing" ;
	rdfs:seeAlso <https://github.com/ethereum/wiki/wiki/White-Paper> ;
	dc:contributor "Joseph Chow" ;
	rdfs:comment "The EthOn Ethereum ontology, described using W3C RDF Schema and the Web Ontology Language. It is closely aligned with Gavin Wood's Ethereum yellow paper."@en ;
	dc:contributor "Casey Detrio" , "Maurycy Pietrzak" , "Alex Beregszazi" ;
	rdfs:seeAlso <https://github.com/ConsenSys/EthOn> ;
	dc:title "EthOn - An Ethereum Ontology" ;
	dc:contributor "Herman Junge" ;
	owl:versionInfo "0.2" ;
	vann:preferredNamespacePrefix "ethon" ;
	dc:contributor "William E Bodell III" , "Stefano Bertolo" , "Marian Oancea" .
# 
# 
# #################################################################
# #
# #    Annotation properties
# #
# #################################################################
# 
# 
# http://ethon.consensys.net/EthOnAnnotationProperty

:EthOnAnnotationProperty a owl:AnnotationProperty ;
	rdfs:comment "Superclass of all EthOn specific annotation properties."@en ;
	ns:term_status "unstable" .
# 
# http://ethon.consensys.net/simpleDefinition

:simpleDefinition a owl:AnnotationProperty ;
	rdfs:comment "This property relates an EthOn concept to a definition in Simple English, intended especially for non-technical users." ;
	ns:term_status "unstable" ;
	rdfs:subPropertyOf :EthOnAnnotationProperty ;
	rdfs:domain :EthOnConcept .
# 
# http://ethon.consensys.net/suggestedStringRepresentation

:suggestedStringRepresentation a owl:AnnotationProperty ;
	rdfs:comment "This property relates an EthOn concept with a suggested string representation. It can be used to give the term a name, e.g. in program code."@en ;
	ns:term_status "unstable" ;
	rdfs:subPropertyOf :EthOnAnnotationProperty ;
	rdfs:domain :EthOnConcept .
# 
# 
# 
# #################################################################
# #
# #    Object Properties
# #
# #################################################################
# 
# 
# http://ethon.consensys.net/AccountObjectProperty

:AccountObjectProperty a owl:ObjectProperty ;
	rdfs:subPropertyOf :EthOnObjectProperty ;
	rdfs:comment "Groups all EthOn account object properties"@en ;
	rdfs:label "EthOn Account Object Property"@en ;
	ns:term_status "unstable" .
# 
# http://ethon.consensys.net/BlockObjectProperty

:BlockObjectProperty a owl:ObjectProperty ;
	rdfs:subPropertyOf :EthOnObjectProperty ;
	rdfs:comment "Groups all EthOn block object properties"@en ;
	rdfs:label "EthOn Block Object Property"@en ;
	ns:term_status "unstable" .
# 
# http://ethon.consensys.net/EthOnObjectProperty

:EthOnObjectProperty a owl:ObjectProperty ;
	rdfs:comment "Groups all EthOn object properties"@en ;
	rdfs:label "EthOn Object Property"@en ;
	ns:term_status "unstable" .
# 
# http://ethon.consensys.net/MessageObjectProperty

:MessageObjectProperty a owl:ObjectProperty ;
	rdfs:subPropertyOf :EthOnObjectProperty ;
	rdfs:comment "Groups all EthOn message object properties."@en ;
	rdfs:label "EthOn Message Object Property"@en ;
	ns:term_status "unstable" .
# 
# http://ethon.consensys.net/NetworkObjectProperty

:NetworkObjectProperty a owl:ObjectProperty ;
	rdfs:subPropertyOf :EthOnObjectProperty ;
	rdfs:comment "Groups all EthOn network object properties."@en ;
	rdfs:label "EthOn Network Object Property"@en ;
	ns:term_status "unstable" .
# 
# http://ethon.consensys.net/StateObjectProperty

:StateObjectProperty a owl:ObjectProperty ;
	rdfs:subPropertyOf :EthOnObjectProperty ;
	rdfs:comment "Groups all EthOn state object properties."@en ;
	rdfs:label "EthOn State Object Property"@en ;
	ns:term_status "unstable" .
# 
# http://ethon.consensys.net/conformsTo

:conformsTo a owl:ObjectProperty ;
	rdfs:subPropertyOf :NetworkObjectProperty ;
	rdfs:domain :Block ;
	rdfs:range :ProtocolVariant ;
	:suggestedStringRepresentation "conformsTo" ;
	rdfs:comment "Relates a Block to the protocol variant it conforms to."@en ;
	rdfs:label "conforms to" ;
	ns:term_status "unstable" .
# 
# http://ethon.consensys.net/containsBlock

:containsBlock a owl:ObjectProperty ;
	rdfs:subPropertyOf :NetworkObjectProperty ;
	rdfs:domain :Blockchain ;
	rdfs:range :Block ;
	:suggestedStringRepresentation "containsBlock" ;
	rdfs:comment "Relates an Ethereum Blockchain to a Block that it contains."@en ;
	rdfs:label "contains Block" ;
	ns:term_status "unstable" .
# 
# http://ethon.consensys.net/containsCanonicalBlock

:containsCanonicalBlock a owl:ObjectProperty ;
	rdfs:subPropertyOf :containsBlock ;
	rdfs:domain :Blockchain ;
	rdfs:range :Block ;
	:suggestedStringRepresentation "containsCanonicalBlock" ;
	rdfs:comment "Relates a blockchain to a canonical block that it contains. A canonical Block is the first block in a blockchain after a fork and that conforms to a new protocol variant."@en ;
	rdfs:label "contains canonical Block" ;
	ns:term_status "unstable" .
# 
# http://ethon.consensys.net/containsTx

:containsTx a owl:ObjectProperty ;
	rdfs:subPropertyOf :BlockObjectProperty ;
	a owl:InverseFunctionalProperty ;
	rdfs:domain :Block ;
	rdfs:range :Tx ;
	:suggestedStringRepresentation "containsTx" ;
	rdfs:comment "Relates a block to a transaction included in it. All containsTx relations of a block comprise the block's transaction list. The order of the transactions is determined by their index value. The property is inverse functional because a transaction can only be included in one block."@en ;
	rdfs:label "contains Transaction"@en ;
	ns:term_status "unstable" .
# 
# http://ethon.consensys.net/controlsAccount

:controlsAccount a owl:ObjectProperty ;
	rdfs:subPropertyOf :AccountObjectProperty ;
	rdfs:domain :ExternalActor ;
	rdfs:range :Account ;
	:suggestedStringRepresentation "controlsAccount" ;
	rdfs:comment "This property connects an External Actor an Account that it controls. This means the External Actor has control over the private Key for the Account. The control is not necessarily legitimate."@en ;
	rdfs:label "controls Account"@en ;
	ns:term_status "unstable" .
# 
# http://ethon.consensys.net/creates

:creates a owl:ObjectProperty ;
	rdfs:subPropertyOf :to ;
	rdfs:domain _:genid1 .

_:genid1 a owl:Class ;
	owl:unionOf _:genid3 .

_:genid3 a rdf:List ;
	rdf:first :CreateContractMsg ;
	rdf:rest _:genid2 .

_:genid2 a rdf:List ;
	rdf:first :CreateTx ;
	rdf:rest rdf:nil .

:creates rdfs:range :ContractAccount ;
	:suggestedStringRepresentation "creates" ;
	rdfs:comment "Relates a create message to the contract account it creates. Note: this is a subproperty of the to property."@en ;
	rdfs:label "creates"@en ;
	ns:term_status "unstable" .
# 
# http://ethon.consensys.net/createsPostBlockState

:createsPostBlockState a owl:ObjectProperty ;
	rdfs:subPropertyOf :createsState ;
	a owl:FunctionalProperty , owl:InverseFunctionalProperty ;
	rdfs:domain :Block ;
	rdfs:range :WorldState ;
	:suggestedStringRepresentation "createsPostBlockState" ;
	rdfs:comment "Relates a block to the global state of the system after all transactions in the block have been executed."@en ;
	rdfs:label "creates post Block execution State"@en ;
	ns:term_status "unstable" .
# 
# http://ethon.consensys.net/createsPostMsgState

:createsPostMsgState a owl:ObjectProperty ;
	rdfs:subPropertyOf :createsState ;
	a owl:FunctionalProperty ;
	rdfs:comment "Relates a message to the global state of the system after all the message has been executed." ;
	rdfs:label "creates post Message execution State" ;
	ns:term_status "unstable" .
# 
# http://ethon.consensys.net/createsPostTxState

:createsPostTxState a owl:ObjectProperty ;
	rdfs:subPropertyOf :createsState ;
	a owl:FunctionalProperty ;
	rdfs:domain :Tx ;
	rdfs:range :WorldState ;
	:suggestedStringRepresentation "createsPostTxState" ;
	rdfs:comment "Relates a transaction to the global state of the system after the transaction has been executed."@en ;
	rdfs:label "creates post Transaction execution State"@en ;
	ns:term_status "unstable" .
# 
# http://ethon.consensys.net/createsState

:createsState a owl:ObjectProperty ;
	rdfs:subPropertyOf :MessageObjectProperty , :StateObjectProperty ;
	rdfs:domain :StateTransition ;
	rdfs:range :State ;
	:suggestedStringRepresentation "createsState" ;
	rdfs:comment "Relates a transition to the state it creates."@en ;
	rdfs:label "creates State"@en ;
	ns:term_status "unstable" .
# 
# http://ethon.consensys.net/from

:from a owl:ObjectProperty ;
	rdfs:subPropertyOf :MessageObjectProperty ;
	owl:inverseOf :sends ;
	rdfs:domain :Msg ;
	rdfs:range :Account ;
	:suggestedStringRepresentation "fromAccount" ;
	rdfs:comment "Relates a message to the account it originates from."@en ;
	rdfs:label "from"@en ;
	ns:term_status "unstable" .
# 
# http://ethon.consensys.net/hasAccountStorage

:hasAccountStorage a owl:ObjectProperty ;
	rdfs:subPropertyOf :AccountObjectProperty ;
	a owl:FunctionalProperty , owl:InverseFunctionalProperty ;
	rdfs:range :AccountStorage ;
	:suggestedStringRepresentation "hasAccountStorage" ;
	rdfs:comment "Relates an account to the Merkle Patricia tree that encodes its storage contents at a certain account state. This property is Functional because an account state can have only one instance of account storage and inverse functional because an account storage can have only one associated account state."@en ;
	rdfs:label "has Account Storage"@en ;
	ns:term_status "unstable" .
# 
# http://ethon.consensys.net/hasAuthorBeneficiary

:hasAuthorBeneficiary a owl:ObjectProperty ;
	rdfs:subPropertyOf :hasBeneficiary ;
	a owl:FunctionalProperty ;
	rdfs:domain :Block ;
	rdfs:range :Account ;
	:suggestedStringRepresentation "hasAuthorBeneficiary" ;
	rdfs:comment "Relates a block to an account to which the fees from gas costs, the static mining reward and the reward for including uncles are transferred." ;
	rdfs:label "has author beneficiary" ;
	ns:term_status "unstable" .
# 
# http://ethon.consensys.net/hasBeneficiary

:hasBeneficiary a owl:ObjectProperty ;
	rdfs:subPropertyOf :BlockObjectProperty ;
	rdfs:domain :Block ;
	rdfs:range :Account ;
	:suggestedStringRepresentation "hasBeneficiary" ;
	rdfs:comment "Relates a block to an account to which fees or mining rewards from the successful mining of this block are transferred."@en ;
	rdfs:label "has beneficiary"@en ;
	ns:term_status "unstable" .
# 
# http://ethon.consensys.net/hasBilateralFork

:hasBilateralFork a owl:ObjectProperty ;
	rdfs:subPropertyOf :hasFork ;
	a owl:InverseFunctionalProperty , owl:AsymmetricProperty , owl:TransitiveProperty , owl:IrreflexiveProperty ;
	rdfs:domain :ProtocolVariant ;
	rdfs:range :ProtocolVariant ;
	:suggestedStringRepresentation "hasBilateralFork" ;
	rdfs:comment "Relates a protocol variant to a bilaterally forked version of it. In contrast to a hard fork, a bilateral fork may expand some rules and make others more strict. While in a hard fork rules are expanded only and all pre-fork blocks also comply to the new rules, after a bilateral hard fork, pre-fork some blocks may not be compliant to new protocol."@en ;
	rdfs:label "has bilateral Fork"@en ;
	ns:term_status "unstable" .
# 
# http://ethon.consensys.net/hasCurrentState

:hasCurrentState a owl:ObjectProperty ;
	rdfs:subPropertyOf :hasState ;
	a owl:InverseFunctionalProperty ;
	rdfs:domain :Account ;
	rdfs:range :AccountState ;
	:suggestedStringRepresentation "hasCurrentState" ;
	rdfs:comment "This property relates an EthOn concept to its most current state." ;
	rdfs:label "has current State" ;
	ns:term_status "unstable" .
# 
# http://ethon.consensys.net/hasFork

:hasFork a owl:ObjectProperty ;
	rdfs:subPropertyOf :NetworkObjectProperty ;
	a owl:InverseFunctionalProperty , owl:AsymmetricProperty , owl:TransitiveProperty , owl:IrreflexiveProperty ;
	rdfs:domain :ProtocolVariant ;
	rdfs:range :ProtocolVariant ;
	:suggestedStringRepresentation "hasFork" ;
	rdfs:comment """Relates a protocol variant to a forked version of it. A fork in a protocol variant is a change of the rules for creating valid new blocks (the protocol).

It is inverse functional because a forked protocol can have only one protocol variant it forked from. It is transitive because if a protocol C that was forked from protocol B that in turn was forked from protocol A, protocol C was also forked from protocol A. It is asymetric because if protocol A is forked from protocol B, B cannot be also forked from A. It is irreflexive because a protocol cannot be a fork of itself."""@en ;
	rdfs:label "has Fork"@en ;
	rdfs:seeAlso <http://vitalik.ca/general/2017/03/14/forks_and_markets.html> ;
	ns:term_status "unstable" .
# 
# http://ethon.consensys.net/hasHardFork

:hasHardFork a owl:ObjectProperty ;
	rdfs:subPropertyOf :hasFork ;
	a owl:InverseFunctionalProperty , owl:AsymmetricProperty , owl:TransitiveProperty , owl:IrreflexiveProperty ;
	rdfs:domain :ProtocolVariant ;
	rdfs:range :ProtocolVariant ;
	:suggestedStringRepresentation "hasSoftFork" ;
	rdfs:comment "Relates a protocol variant to a hard forked version of it. Hard forks expand the rule set of a protocol variant or change it incompatibly. Users who want to be on the hard forked chain have to update their clients."@en ;
	rdfs:label "has hard Fork"@en ;
	ns:term_status "unstable" .
# 
# http://ethon.consensys.net/hasLogEntry

:hasLogEntry a owl:ObjectProperty ;
	rdfs:subPropertyOf :MessageObjectProperty ;
	rdfs:domain :Tx ;
	rdfs:range :LogEntry ;
	:suggestedStringRepresentation "hasLogEntry" ;
	rdfs:comment "Relates a transaction to a log entry it creates."@en ;
	rdfs:label "has Log Entry"@en ;
	ns:term_status "unstable" .
# 
# http://ethon.consensys.net/hasLogTopic

:hasLogTopic a owl:ObjectProperty ;
	rdfs:subPropertyOf :MessageObjectProperty ;
	rdfs:domain :LogEntry ;
	rdfs:range :LogTopic ;
	:suggestedStringRepresentation "hasLogTopic" ;
	rdfs:comment "Relates a log entry to a log topic."@en ;
	rdfs:label "has Log Topic"@en ;
	ns:term_status "unstable" .
# 
# http://ethon.consensys.net/hasOriginatorTx

:hasOriginatorTx a owl:ObjectProperty ;
	rdfs:subPropertyOf :MessageObjectProperty ;
	a owl:InverseFunctionalProperty ;
	rdfs:domain :ContractMsg ;
	rdfs:range :Tx ;
	:suggestedStringRepresentation "hasOriginatorTx" ;
	rdfs:comment "Relates a contract message to the transaction it originated from."@en ;
	rdfs:label "has Originator Transaction"@en ;
	ns:term_status "unstable" .
# 
# http://ethon.consensys.net/hasParentBlock

:hasParentBlock a owl:ObjectProperty ;
	rdfs:subPropertyOf :BlockObjectProperty ;
	a owl:FunctionalProperty , owl:AsymmetricProperty , owl:IrreflexiveProperty ;
	rdfs:domain :Block ;
	rdfs:range :Block ;
	:suggestedStringRepresentation "hasParentBlock" ;
	rdfs:comment "Relates a block to its parent in the chain. It always points to the block with a number that is decreased by one, compared to the block it originates from. The relation is asymmetric because if block A is parent to block B then block B can not be parent to block A. It is also irreflexive because a block cannot be parent to itself."@en ;
	rdfs:label "has parent Block"@en ;
	ns:term_status "unstable" .
# 
# http://ethon.consensys.net/hasReceipt

:hasReceipt a owl:ObjectProperty ;
	rdfs:subPropertyOf :MessageObjectProperty ;
	rdfs:domain :Tx ;
	rdfs:range :TxReceipt ;
	:suggestedStringRepresentation "hasTransactionReceipt" ;
	rdfs:comment "Relates a transaction to its receipt."@en ;
	rdfs:label "has transaction receipt"@en ;
	ns:term_status "unstable" .
# 
# http://ethon.consensys.net/hasReceiptsTrie

:hasReceiptsTrie a owl:ObjectProperty ;
	rdfs:subPropertyOf :BlockObjectProperty ;
	a owl:FunctionalProperty , owl:InverseFunctionalProperty ;
	rdfs:domain :Block ;
	rdfs:range :ReceiptsTrie ;
	:suggestedStringRepresentation "hasReceiptsTrie" ;
	rdfs:comment "Relates a block to the trie that contains the block's receipt data."@en ;
	rdfs:label "has receipts trie"@en ;
	ns:term_status "unstable" .
# 
# http://ethon.consensys.net/hasSoftFork

:hasSoftFork a owl:ObjectProperty ;
	rdfs:subPropertyOf :hasFork ;
	a owl:InverseFunctionalProperty , owl:AsymmetricProperty , owl:TransitiveProperty , owl:IrreflexiveProperty ;
	rdfs:domain :ProtocolVariant ;
	rdfs:range :ProtocolVariant ;
	:suggestedStringRepresentation "hasSoftFork" ;
	rdfs:comment "Relates a protocol variant to a soft forked version of it. Soft forks make the rules of a protocol variant more strict. Blocks in the soft forked chain conform to multiple protocol versions at the same time."@en ;
	rdfs:label "has soft Fork"@en ;
	ns:term_status "unstable" .
# 
# http://ethon.consensys.net/hasState

:hasState a owl:ObjectProperty ;
	rdfs:subPropertyOf :StateObjectProperty ;
	a owl:InverseFunctionalProperty ;
	rdfs:domain :Account ;
	rdfs:range :AccountState ;
	:suggestedStringRepresentation "hasState" ;
	rdfs:comment "This property relates an EthOn concept to a state. It is inverse functional because a state can only belong to one single EthOn concept."@en ;
	rdfs:label "has state"@en ;
	ns:term_status "unstable" .
# 
# http://ethon.consensys.net/hasTransition

:hasTransition a owl:ObjectProperty ;
	rdfs:subPropertyOf :StateObjectProperty ;
	:suggestedStringRepresentation "hasTransition" ;
	rdfs:comment "Relates a state to a transition (i.e. a message) that creates a new state."@en ;
	rdfs:label "has Transition"@en ;
	ns:term_status "unstable" .
# 
# http://ethon.consensys.net/hasTxTrie

:hasTxTrie a owl:ObjectProperty ;
	rdfs:subPropertyOf :BlockObjectProperty ;
	a owl:FunctionalProperty , owl:InverseFunctionalProperty ;
	rdfs:domain :Block ;
	rdfs:range :TxTrie ;
	:suggestedStringRepresentation "hasTxTrie" ;
	rdfs:comment "Relates a block to the trie that contains the data of the transactions contained in the block."@en ;
	rdfs:label "has transactions trie"@en ;
	ns:term_status "unstable" .
# 
# http://ethon.consensys.net/hasUncleBeneficiary

:hasUncleBeneficiary a owl:ObjectProperty ;
	rdfs:subPropertyOf :hasBeneficiary ;
	rdfs:domain :Block ;
	rdfs:range :Account ;
	:suggestedStringRepresentation "hasUncleBeneficiary" ;
	rdfs:comment "Relates a block to an account to which the reward for mining an uncle is transferred." ;
	rdfs:label "has uncle beneficiary" ;
	ns:term_status "unstable" .
# 
# http://ethon.consensys.net/includesUncle

:includesUncle a owl:ObjectProperty ;
	rdfs:subPropertyOf :BlockObjectProperty ;
	rdfs:domain :Block ;
	rdfs:range :Uncle ;
	:suggestedStringRepresentation "includesUncle" ;
	rdfs:comment "Relates a block to another block by including it as an uncle. Block B can be an uncle of block A if it is the direct child of the k'th generation ancestor of block B, where 2<=k<=7 but not a direct ancestor of block A. Uncles are blocks found by a miner, when a different miner has already found another block for the corresponding place in the blockchain. They are also known as “stale blocks”."@en ;
	rdfs:label "includes Uncle"@en ;
	ns:term_status "unstable" .
# 
# http://ethon.consensys.net/loggedBy

:loggedBy a owl:ObjectProperty ;
	rdfs:subPropertyOf :MessageObjectProperty ;
	rdfs:domain :LogEntry ;
	rdfs:range :Account ;
	:suggestedStringRepresentation "loggedBy" ;
	rdfs:comment "Relates a log entry to the contract account that created the log when its code was executed."@en ;
	rdfs:label "logged by"@en ;
	ns:term_status "unstable" .
# 
# http://ethon.consensys.net/minesFor

:minesFor a owl:ObjectProperty ;
	rdfs:subPropertyOf :NetworkObjectProperty ;
	rdfs:domain :Node ;
	rdfs:range :Blockchain ;
	:suggestedStringRepresentation "minesFor" ;
	rdfs:comment "Relates a mining node to the blockchain it mines for. Mining is the process of dedicating effort (working) to bolster one series of transactions (a block) over any other potential competitor block. It is achieved thanks to a cryptographically secure proof."@en ;
	rdfs:label "mines for"@en ;
	ns:term_status "unstable" .
# 
# http://ethon.consensys.net/nextBlockState

:nextBlockState a owl:ObjectProperty ;
	rdfs:subPropertyOf :nextTxState ;
	rdfs:domain :PostBlockState ;
	rdfs:range :PostBlockState ;
	:suggestedStringRepresentation "nextBlockState" ;
	rdfs:comment "Relates a post block state to the following post block state."@en ;
	rdfs:label "next Post Block State"@en ;
	ns:term_status "unstable" .
# 
# http://ethon.consensys.net/nextMsgState

:nextMsgState a owl:ObjectProperty ;
	rdfs:subPropertyOf :nextState ;
	rdfs:domain :PostMsgState ;
	rdfs:range :PostMsgState ;
	:suggestedStringRepresentation "nextMsgState" ;
	rdfs:comment "Relates a post message state to the following post message state."@en ;
	rdfs:label "next Post Message State"@en ;
	ns:term_status "unstable" .
# 
# http://ethon.consensys.net/nextState

:nextState a owl:ObjectProperty ;
	rdfs:subPropertyOf :StateObjectProperty ;
	rdfs:domain :WorldState ;
	rdfs:range :WorldState ;
	:suggestedStringRepresentation "nextState" ;
	rdfs:comment "Relates a state to the following state. In EthOn the state transition system has no branches."@en ;
	rdfs:label "next State"@en ;
	ns:term_status "unstable" .
# 
# http://ethon.consensys.net/nextTxState

:nextTxState a owl:ObjectProperty ;
	rdfs:subPropertyOf :nextMsgState ;
	rdfs:domain :PostTxState ;
	rdfs:range :PostTxState ;
	:suggestedStringRepresentation "nextTxState" ;
	rdfs:comment "Relates a post transaction state to the following post transaction state."@en ;
	rdfs:label "next Post Transaction State"@en ;
	ns:term_status "unstable" .
# 
# http://ethon.consensys.net/partOf

:partOf a owl:ObjectProperty ;
	rdfs:subPropertyOf :EthOnObjectProperty ;
	a owl:TransitiveProperty ;
	:suggestedStringRepresentation "partOf" ;
	rdfs:comment "This is a general relation to express part of relationships. The classic study of parts and wholes, mereology, has three axioms: 1. the part-of relation is Transitive - \"parts of parts are parts of the whole\" - If A is part of B and B is part of C, then A is part of C Reflexive - \"Everything is part of itself\" - A is part of A Antisymmetric - \"Nothing is a part of its parts\" - if A is part of B and A != B then B is not part of A."@en ;
	rdfs:label "part of"@en ;
	rdfs:seeAlso <https://www.w3.org/2001/sw/BestPractices/OEP/SimplePartWhole/> ;
	ns:term_status "testing" .
# 
# http://ethon.consensys.net/refunds

:refunds a owl:ObjectProperty ;
	rdfs:subPropertyOf :to ;
	a owl:FunctionalProperty ;
	rdfs:domain :ContractAccount ;
	rdfs:range :Account ;
	:suggestedStringRepresentation "refunds" ;
	rdfs:comment "Relates a selfdestruct contract message to the contract account it sends its refund balance to."@en ;
	rdfs:label "refunds"@en ;
	ns:term_status "unstable" .
# 
# http://ethon.consensys.net/sends

:sends a owl:ObjectProperty ;
	rdfs:subPropertyOf :MessageObjectProperty ;
	rdfs:domain :Account ;
	rdfs:range :Msg ;
	:suggestedStringRepresentation "sends" ;
	rdfs:comment "Relates a an account to a message it sends."@en ;
	rdfs:label "sends"@en ;
	ns:term_status "unstable" .
# 
# http://ethon.consensys.net/spawnsBlock

:spawnsBlock a owl:ObjectProperty ;
	rdfs:subPropertyOf :NetworkObjectProperty ;
	rdfs:domain :Node ;
	rdfs:range :Block ;
	:suggestedStringRepresentation "spawnsBlock" ;
	rdfs:comment "Relates an Ethereum node to a valid block it has transmitted to the network. This does not specify the proofing algorithm (e.g. proof of work or proof of authority)."@en ;
	rdfs:label "spawns Block" ;
	ns:term_status "unstable" .
# 
# http://ethon.consensys.net/to

:to a owl:ObjectProperty ;
	rdfs:subPropertyOf :MessageObjectProperty ;
	rdfs:domain :Msg ;
	rdfs:range :Account ;
	:suggestedStringRepresentation "toAccount" ;
	rdfs:comment "Relates a message with the account it is sent to."@en ;
	rdfs:label "to"@en ;
	ns:term_status "unstable" .
# 
# http://ethon.consensys.net/triggersMsg

:triggersMsg a owl:ObjectProperty ;
	rdfs:subPropertyOf :MessageObjectProperty ;
	rdfs:domain _:genid4 .

_:genid4 a owl:Class ;
	owl:unionOf _:genid8 .

_:genid8 a rdf:List ;
	rdf:first :CallContractMsg ;
	rdf:rest _:genid7 .

_:genid7 a rdf:List ;
	rdf:first :CallTx ;
	rdf:rest _:genid6 .

_:genid6 a rdf:List ;
	rdf:first :CreateContractMsg ;
	rdf:rest _:genid5 .

_:genid5 a rdf:List ;
	rdf:first :CreateTx ;
	rdf:rest rdf:nil .

:triggersMsg rdfs:range :ContractMsg ;
	:suggestedStringRepresentation "triggersMsg" ;
	rdfs:comment "Relates a message that was directed to a contract account to the contract messages that result from it. The chain of triggersMsg relations represents a call tree. The messages related to a message via triggersMsg are the direct children of it in the call tree."@en ;
	rdfs:label "triggers Contract Message"@en ;
	ns:term_status "unstable" .
# 
# 
# 
# #################################################################
# #
# #    Data properties
# #
# #################################################################
# 
# 
# http://ethon.consensys.net/AccountDataProperty

:AccountDataProperty a owl:DatatypeProperty ;
	rdfs:subPropertyOf :EthOnDataProperty ;
	rdfs:domain :AccountConcept ;
	rdfs:comment "Groups all data properties that are specific to an account."@en ;
	rdfs:label "EthOn Account Data Property"@en ;
	ns:term_status "unstable" .
# 
# http://ethon.consensys.net/BlockDataProperty

:BlockDataProperty a owl:DatatypeProperty ;
	rdfs:subPropertyOf :EthOnDataProperty ;
	rdfs:domain :BlockConcept ;
	rdfs:comment "Groups all data properties that are specific to a block. These properties are usually functional because a block can only be associated with a single instance of them."@en ;
	rdfs:label "EthOn Block Data Property"@en ;
	ns:term_status "unstable" .
# 
# http://ethon.consensys.net/EthOnDataProperty

:EthOnDataProperty a owl:DatatypeProperty ;
	rdfs:subPropertyOf owl:topDataProperty ;
	rdfs:comment "Groups all data properties specific to EthOn."@en ;
	rdfs:label "EthOn Data Property"@en ;
	ns:term_status "unstable" .
# 
# http://ethon.consensys.net/MessageDataProperty

:MessageDataProperty a owl:DatatypeProperty ;
	rdfs:subPropertyOf :EthOnDataProperty ;
	rdfs:domain :MessageConcept ;
	rdfs:comment "Groups all EthOn message data properties."@en ;
	rdfs:label "EthOn Message Data Property" ;
	ns:term_status "unstable" .
# 
# http://ethon.consensys.net/NetworkDataProperty

:NetworkDataProperty a owl:DatatypeProperty ;
	rdfs:subPropertyOf :EthOnDataProperty ;
	rdfs:comment "Groups all EthOn network data properties."@en ;
	rdfs:label "EthOn Network Data Property"@en ;
	ns:term_status "unstable" .
# 
# http://ethon.consensys.net/StateDataProperty

:StateDataProperty a owl:DatatypeProperty ;
	rdfs:subPropertyOf :EthOnDataProperty ;
	rdfs:domain :StateConcept .
# 
# http://ethon.consensys.net/accountBalance

:accountBalance a owl:DatatypeProperty ;
	rdfs:subPropertyOf :AccountDataProperty ;
	a owl:FunctionalProperty ;
	rdfs:domain :AccountState ;
	rdfs:range xsd:integer ;
	:suggestedStringRepresentation "accountBalance" ;
	rdfs:comment "A scalar value equal to the number of Wei owned by an account at a given account state."@en ;
	rdfs:label "Account balance"@en ;
	ns:term_status "unstable" .
# 
# http://ethon.consensys.net/accountBalancePrefunded

:accountBalancePrefunded a owl:DatatypeProperty ;
	rdfs:subPropertyOf :AccountDataProperty ;
	rdfs:domain :ProtocolAccount ;
	rdfs:range xsd:integer ;
	:suggestedStringRepresentation "accountBalancePrefunded" ;
	rdfs:comment "The amount of Wei an account was prefunded with in a protocol variant. In the case that an account receives multiple prefunds in multiple protocol variants, the amounts are summed. In contrast to the regular account balance it is a property of the account itself and not of its state."@en ;
	rdfs:label "Account balance prefunded"@en ;
	ns:term_status "unstable" .
# 
# http://ethon.consensys.net/accountCode

:accountCode a owl:DatatypeProperty ;
	rdfs:subPropertyOf :AccountDataProperty ;
	a owl:FunctionalProperty ;
	rdfs:domain :ContractAccount ;
	rdfs:range xsd:hexBinary ;
	:suggestedStringRepresentation "accountCode" ;
	rdfs:comment "The immutable EVM bytecode of the contract account."@en ;
	rdfs:label "Account code"@en ;
	ns:term_status "unstable" .
# 
# http://ethon.consensys.net/accountCodeHash

:accountCodeHash a owl:DatatypeProperty ;
	rdfs:subPropertyOf :AccountDataProperty ;
	a owl:FunctionalProperty ;
	rdfs:domain :ContractAccount ;
	rdfs:range xsd:hexBinary ;
	:suggestedStringRepresentation "accountCodeHash" ;
	rdfs:comment "The immutable Keccak-256 hash of the EVM code of an account."@en ;
	rdfs:label "Account code hash"@en ;
	ns:term_status "unstable" .
# 
# http://ethon.consensys.net/accountNonce

:accountNonce a owl:DatatypeProperty ;
	rdfs:subPropertyOf :AccountDataProperty ;
	a owl:FunctionalProperty ;
	rdfs:domain :AccountState ;
	rdfs:range xsd:integer ;
	:suggestedStringRepresentation "accountNonce" ;
	rdfs:comment "A scalar value equal to the number of transactions sent from this account or, in the case of accounts with associated code, the number of contract-creations made by this account."@en ;
	rdfs:label "Account nonce"@en ;
	ns:term_status "unstable" .
# 
# http://ethon.consensys.net/accountPublicKey

:accountPublicKey a owl:DatatypeProperty ;
	rdfs:subPropertyOf :AccountDataProperty ;
	a owl:FunctionalProperty ;
	rdfs:domain :ExternalAccount ;
	rdfs:range xsd:hexBinary ;
	:suggestedStringRepresentation "accountPublicKey" ;
	rdfs:comment "The public key of an external account."@en ;
	rdfs:label "Account public key"@en ;
	ns:term_status "unstable" .
# 
# http://ethon.consensys.net/address

:address a owl:DatatypeProperty ;
	rdfs:subPropertyOf :AccountDataProperty ;
	a owl:FunctionalProperty ;
	rdfs:domain :Account ;
	rdfs:range xsd:hexBinary ;
	:suggestedStringRepresentation "address" ;
	rdfs:comment "A 160-bit identifier for accounts."@en ;
	rdfs:label "Address"@en ;
	ns:term_status "unstable" .
# 
# http://ethon.consensys.net/blockBeneficiaryReward

:blockBeneficiaryReward a owl:DatatypeProperty ;
	rdfs:subPropertyOf :BlockDataProperty ;
	a owl:FunctionalProperty ;
	rdfs:domain :Block ;
	rdfs:range xsd:integer ;
	:suggestedStringRepresentation "blockBenficiaryReward" ;
	rdfs:comment "The reward the beneficiary receives for mining a block. It is comprised of the base reward (5ETH), rewards for including uncles (1/32 of block reward per uncle) and the fees of the Tx in the block."@en ;
	rdfs:label "Block beneficiary reward"@en ;
	ns:term_status "unstable" .
# 
# http://ethon.consensys.net/blockCreationTime

:blockCreationTime a owl:DatatypeProperty ;
	rdfs:subPropertyOf :BlockDataProperty ;
	a owl:FunctionalProperty ;
	rdfs:domain :Block ;
	rdfs:range xsd:dateTime ;
	:suggestedStringRepresentation "blockCreationTime" ;
	rdfs:comment "This block's inception date and time."@en ;
	rdfs:label "Block creation time"@en ;
	ns:term_status "unstable" .
# 
# http://ethon.consensys.net/blockDifficulty

:blockDifficulty a owl:DatatypeProperty ;
	rdfs:subPropertyOf :BlockDataProperty ;
	a owl:FunctionalProperty ;
	rdfs:domain :Block ;
	rdfs:range xsd:integer ;
	:suggestedStringRepresentation "blockDifficulty" ;
	rdfs:comment "The difficulty level of this block."@en ;
	rdfs:label "Block difficulty"@en ;
	ns:term_status "unstable" .
# 
# http://ethon.consensys.net/totalBlockDifficulty

:totalBlockDifficulty a owl:DatatypeProperty ;
	rdfs:subPropertyOf :BlockDataProperty ;
	a owl:FunctionalProperty ;
	rdfs:domain :Block ;
	rdfs:range xsd:integer ;
	:suggestedStringRepresentation "totalBlockDifficulty" ;
	rdfs:comment "The difficulty of the total chain until this block."@en ;
	rdfs:label "Total block difficulty"@en ;
	ns:term_status "unstable" .
# 
# http://ethon.consensys.net/blockExtraData

:blockExtraData a owl:DatatypeProperty ;
	rdfs:subPropertyOf :BlockDataProperty ;
	a owl:FunctionalProperty ;
	rdfs:domain :Block ;
	rdfs:range xsd:hexBinary ;
	:suggestedStringRepresentation "blockExtraData" ;
	rdfs:comment "An arbitrary byte array containing data relevant to this block. This must be 32 bytes or fewer."@en ;
	rdfs:label "Block extra data"@en ;
	ns:term_status "unstable" .
# 
# http://ethon.consensys.net/blockGasLimit

:blockGasLimit a owl:DatatypeProperty ;
	rdfs:subPropertyOf :BlockDataProperty ;
	a owl:FunctionalProperty ;
	rdfs:domain :Block ;
	rdfs:range xsd:integer ;
	:suggestedStringRepresentation "blockGasLimit" ;
	rdfs:comment "A scalar value equal to the current limit of gas expenditure per block.  Its purpose is to keep block propagation and processing time low, thereby allowing for a sufficiently decentralized network. Miners have the option to increase or decrease it every block by a certain factor."@en ;
	rdfs:label "Block gas limit"@en ;
	ns:term_status "unstable" .
# 
# http://ethon.consensys.net/blockGasUsed

:blockGasUsed a owl:DatatypeProperty ;
	rdfs:subPropertyOf :BlockDataProperty ;
	a owl:FunctionalProperty ;
	rdfs:domain :Block ;
	rdfs:range xsd:integer ;
	:suggestedStringRepresentation "blockGasUsed" ;
	rdfs:comment "A scalar value equal to the total gas used by all transactions in this block."@en ;
	rdfs:label "Block gas used"@en ;
	ns:term_status "unstable" .
# 
# http://ethon.consensys.net/blockHash

:blockHash a owl:DatatypeProperty ;
	rdfs:subPropertyOf :BlockDataProperty ;
	a owl:FunctionalProperty ;
	rdfs:domain :Block ;
	rdfs:range xsd:hexBinary ;
	:suggestedStringRepresentation "blockHash" ;
	rdfs:comment "The Keccak 256-bit hash of the block's header, in its entierty."@en ;
	rdfs:label "Block hash"@en ;
	ns:term_status "unstable" .
# 
# http://ethon.consensys.net/blockHeader

:blockHeader a owl:DatatypeProperty ;
	rdfs:subPropertyOf :BlockDataProperty ;
	a owl:FunctionalProperty ;
	rdfs:domain :Block ;
	rdfs:range xsd:hexBinary ;
	:suggestedStringRepresentation "blockHeader" ;
	rdfs:comment "Relates a block to its block header data. The block header data contains 15 pieces of information: 1. the parent hash, 2. the Uncle hash, 3. a beneficiary address, 4. a state root hash, 5. a transactions root hash, 6. a receipts root hash, 7. a log bloom filter, 8. the difficulty value, 9. the block number, 10. the gas limit of the block, 11. the gas used by all transactions in the block, 12. a scalar timestamp in unix time() format, 13. a byte array containing extra data, 14. a mix hash and 15. the block nonce. The property is functional because a block can have only exactly one block header."@en ;
	rdfs:label "Block header"@en ;
	ns:term_status "unstable" .
# 
# http://ethon.consensys.net/blockLogsBloom

:blockLogsBloom a owl:DatatypeProperty ;
	rdfs:subPropertyOf :BlockDataProperty ;
	a owl:FunctionalProperty ;
	rdfs:domain :Block ;
	rdfs:range xsd:hexBinary ;
	:suggestedStringRepresentation "blockLogsBloom" ;
	rdfs:comment """The bloom filter of log entries resulting from the transactions in the block. 

The bloom filter helps to identify blocks with logs quickly. To find the indexed log entries from a contract, only the bloom filters of all blocks, which are included in the block header have to be checked. Note that bloom filters can produce false positives but not false negatives. In other words, if the bloom filter indicates that the topic and contract have not produced any logs in a block, this information is final. If the bloom filter indicates a match, it is only a probabilistic result and has to be verified further. The transactions in the block can then be re-executed and the probabilistic match of the bloom filter can be verified."""@en ;
	rdfs:label "block logs bloom filter"@en ;
	rdfs:seeAlso :txLogsBloom ;
	ns:term_status "unstable" .
# 
# http://ethon.consensys.net/blockMixHash

:blockMixHash a owl:DatatypeProperty ;
	rdfs:subPropertyOf :BlockDataProperty ;
	a owl:FunctionalProperty ;
	rdfs:domain :Block ;
	rdfs:range xsd:hexBinary ;
	:suggestedStringRepresentation "blockMixHash" ;
	rdfs:comment "A 256-bit hash which proves combined with the nonce that a sufficient amount of computation has been carried out on this block."@en ;
	rdfs:label "Block mix hash"@en ;
	ns:term_status "unstable" .
# 
# http://ethon.consensys.net/blockNonce

:blockNonce a owl:DatatypeProperty ;
	rdfs:subPropertyOf :BlockDataProperty ;
	a owl:FunctionalProperty ;
	rdfs:domain :Block ;
	rdfs:range xsd:hexBinary ;
	:suggestedStringRepresentation "blockNonce" ;
	rdfs:comment "A 64 bit hash which proves combined with the mix-hash that a sufficient amount of computation has been carried out on this block."@en ;
	rdfs:label "Block nonce"@en ;
	ns:term_status "unstable" .
# 
# http://ethon.consensys.net/blockSize

:blockSize a owl:DatatypeProperty ;
	rdfs:subPropertyOf :BlockDataProperty ;
	a owl:FunctionalProperty ;
	rdfs:domain :Block ;
	rdfs:range xsd:integer ;
	:suggestedStringRepresentation "blockSize" ;
	rdfs:comment "The size of the block header in RLP format in bytes."@en ;
	rdfs:label "Block size"@en ;
	rdfs:seeAlso <https://github.com/ethereum/wiki/wiki/RLP> ;
	ns:term_status "unstable" .
# 
# http://ethon.consensys.net/clientVersion

:clientVersion a owl:DatatypeProperty ;
	rdfs:subPropertyOf :NetworkDataProperty ;
	rdfs:domain :Node ;
	rdfs:range xsd:string ;
	:suggestedStringRepresentation "clientVersion" ;
	rdfs:comment "Relates a node to a string identifying the Ethereum client version it runs. It composed of the client name (e.g. Geth) and a version identifier (e.g. v1.5.4)."@en ;
	rdfs:label "runs client"@en ;
	ns:term_status "unstable" .
# 
# http://ethon.consensys.net/cumulativeGasUsed

:cumulativeGasUsed a owl:DatatypeProperty ;
	rdfs:subPropertyOf :MessageDataProperty ;
	rdfs:domain :Tx ;
	rdfs:range xsd:integer ;
	:suggestedStringRepresentation "cumulativeGasUsed" ;
	rdfs:comment "The cumulative gas used in the block containing the transaction as of immediately after the transaction has happened."@en ;
	rdfs:label "cumulative gas used"@en ;
	ns:term_status "unstable" .
# 
# http://ethon.consensys.net/logData

:logData a owl:DatatypeProperty ;
	rdfs:subPropertyOf :MessageDataProperty ;
	rdfs:domain :LogEntry ;
	rdfs:range xsd:hexBinary ;
	:suggestedStringRepresentation "logData" ;
	rdfs:comment "Relates a log entry to its data."@en ;
	rdfs:label "Log data"@en ;
	ns:term_status "unstable" .
# 
# http://ethon.consensys.net/logIndex

:logIndex a owl:DatatypeProperty ;
	rdfs:subPropertyOf :MessageDataProperty ;
	a owl:FunctionalProperty ;
	rdfs:domain :Tx ;
	rdfs:range xsd:integer ;
	:suggestedStringRepresentation "logIndex" ;
	rdfs:comment "Relates a log entry to its index in the transaction reciept of a transaction. The log index defines the order of the log entries of a transaction."@en ;
	rdfs:label "Log index"@en ;
	ns:term_status "unstable" .
# 
# http://ethon.consensys.net/logTopicData

:logTopicData a owl:DatatypeProperty ;
	rdfs:subPropertyOf :MessageDataProperty ;
	a owl:FunctionalProperty ;
	rdfs:domain :LogTopic ;
	rdfs:range xsd:hexBinary ;
	:suggestedStringRepresentation "logTopicData" ;
	rdfs:comment "Relates a log topic to the 32 bytes of data it contains."@en ;
	rdfs:label "Log Topic data"@en ;
	ns:term_status "unstable" .
# 
# http://ethon.consensys.net/logTopicIndex

:logTopicIndex a owl:DatatypeProperty ;
	rdfs:subPropertyOf :MessageDataProperty ;
	a owl:FunctionalProperty ;
	rdfs:domain :LogTopic ;
	rdfs:range xsd:integer ;
	:suggestedStringRepresentation "logTopicIndex" ;
	rdfs:comment "Relates a log topic to its index in the log entry. The log topic index defines the order of the log topics of in log entry."@en ;
	rdfs:label "Log Topic index"@en ;
	ns:term_status "unstable" .
# 
# http://ethon.consensys.net/msgCallDepth

:msgCallDepth a owl:DatatypeProperty ;
	rdfs:subPropertyOf :MessageDataProperty ;
	rdfs:domain :Tx ;
	rdfs:range xsd:integer ;
	:suggestedStringRepresentation "msgCallDepth" ;
	rdfs:comment "A scalar value equal to the depth of the contract message. A contract message is represented as a call in the Ethereum EVM. This value represents the number of CALL or CREATE opcodes being executed at the time of the message execution."@en ;
	rdfs:label "Message call depth"@en ;
	ns:term_status "unstable" .
# 
# http://ethon.consensys.net/msgData

:msgData a owl:DatatypeProperty ;
	rdfs:subPropertyOf :msgPayload ;
	rdfs:domain _:genid9 .

_:genid9 a owl:Class ;
	owl:unionOf _:genid11 .

_:genid11 a rdf:List ;
	rdf:first :CallContractMsg ;
	rdf:rest _:genid10 .

_:genid10 a rdf:List ;
	rdf:first :CallTx ;
	rdf:rest rdf:nil .

:msgData rdfs:range xsd:hexBinary ;
	:suggestedStringRepresentation "msgData" ;
	rdfs:comment "An unlimited size byte array specifying the input data of the call."@en ;
	rdfs:label "call data"@en ;
	ns:term_status "unstable" .
# 
# http://ethon.consensys.net/msgError

:msgError a owl:DatatypeProperty ;
	rdfs:subPropertyOf :MessageDataProperty ;
	a owl:FunctionalProperty ;
	rdfs:domain :Msg ;
	rdfs:range xsd:boolean ;
	:suggestedStringRepresentation "msgError" ;
	rdfs:comment "A boolean value indicating whether the message validation resulted in an error. A \"true\" value indicates an error."@en ;
	rdfs:label "Message error"@en ;
	ns:term_status "unstable" .
# 
# http://ethon.consensys.net/msgErrorString

:msgErrorString a owl:DatatypeProperty ;
	rdfs:subPropertyOf :MessageDataProperty ;
	a owl:FunctionalProperty ;
	rdfs:domain :Msg ;
	rdfs:range xsd:string ;
	:suggestedStringRepresentation "msgErrorString" ;
	rdfs:comment "A string informally describing an error that occured during the validation of a message. Only exists if msgError is true."@en ;
	rdfs:label "Message error string"@en ;
	ns:term_status "unstable" .
# 
# http://ethon.consensys.net/msgGasLimit

:msgGasLimit a owl:DatatypeProperty ;
	rdfs:subPropertyOf :MessageDataProperty ;
	rdfs:domain :Msg ;
	rdfs:range xsd:integer ;
	:suggestedStringRepresentation "msgGasLimit" ;
	rdfs:comment "A scalar value equal to the maximum amount of gas that should be used in executing this transaction. This is paid up-front, before any computation is done and may not be increased later. If used with contract messages it represents the fraction of the original transaction gas limit still available for execution of the contract message. After all resulting computations are done, excess gas is returned to the sender of the original transaction."@en ;
	rdfs:label "Message gas limit"@en ;
	ns:term_status "unstable" .
# 
# http://ethon.consensys.net/msgGasUsed

:msgGasUsed a owl:DatatypeProperty ;
	rdfs:subPropertyOf :MessageDataProperty ;
	a owl:FunctionalProperty ;
	rdfs:domain :Msg ;
	rdfs:range xsd:integer ;
	owl:propertyDisjointWith :txGasUsed ;
	:suggestedStringRepresentation "msgGasUsed" ;
	rdfs:comment "The amount of gas that was used for processing a single message, regardless of which type of message it may be."@en ;
	rdfs:label "Msg gas used"@en ;
	ns:term_status "unstable" .
# 
# http://ethon.consensys.net/msgInit

:msgInit a owl:DatatypeProperty ;
	rdfs:subPropertyOf :msgPayload ;
	rdfs:domain _:genid12 .

_:genid12 a owl:Class ;
	owl:unionOf _:genid14 .

_:genid14 a rdf:List ;
	rdf:first :CreateContractMsg ;
	rdf:rest _:genid13 .

_:genid13 a rdf:List ;
	rdf:first :CreateTx ;
	rdf:rest rdf:nil .

:msgInit rdfs:range xsd:hexBinary ;
	:suggestedStringRepresentation "msgInit" ;
	rdfs:comment "An unlimited size byte array specifying the EVM-code for the contract account initialisation procedure."@en ;
	rdfs:label "Message init code"@en ;
	ns:term_status "unstable" .
# 
# http://ethon.consensys.net/msgOutput

:msgOutput a owl:DatatypeProperty ;
	rdfs:subPropertyOf :MessageDataProperty ;
	a owl:FunctionalProperty ;
	rdfs:domain _:genid15 .

_:genid15 a owl:Class ;
	owl:unionOf _:genid17 .

_:genid17 a rdf:List ;
	rdf:first :CallContractMsg ;
	rdf:rest _:genid16 .

_:genid16 a rdf:List ;
	rdf:first :CallTx ;
	rdf:rest rdf:nil .

:msgOutput rdfs:range xsd:hexBinary ;
	:suggestedStringRepresentation "msgOutput" ;
	rdfs:comment "The resulting output data from a call tx or call contract message. This is the return value from the (function) call."@en ;
	rdfs:label "Message output"@en ;
	ns:term_status "unstable" .
# 
# http://ethon.consensys.net/msgPayload

:msgPayload a owl:DatatypeProperty ;
	rdfs:subPropertyOf :MessageDataProperty ;
	a owl:FunctionalProperty ;
	rdfs:domain :Msg ;
	rdfs:range xsd:hexBinary ;
	:suggestedStringRepresentation "msgPayload" ;
	rdfs:comment "An unlimited size byte array specifying the data payload of the message."@en ;
	rdfs:label "Message payload"@en ;
	ns:term_status "unstable" .
# 
# http://ethon.consensys.net/msgRefundBalance

:msgRefundBalance a owl:DatatypeProperty ;
	rdfs:subPropertyOf :MessageDataProperty ;
	a owl:FunctionalProperty ;
	rdfs:domain :SelfdestructContractMsg ;
	rdfs:range xsd:integer ;
	:suggestedStringRepresentation "msgRefundBalance" ;
	rdfs:comment "A scalar value equal to the number of Wei that will be refunded as the result of a selfdestruct contract message."@en ;
	rdfs:label "contract balance in Wei"@en ;
	ns:term_status "unstable" .
# 
# http://ethon.consensys.net/number

:number a owl:DatatypeProperty ;
	rdfs:subPropertyOf :BlockDataProperty ;
	a owl:FunctionalProperty ;
	rdfs:domain :Block ;
	rdfs:range xsd:integer ;
	:suggestedStringRepresentation "number" ;
	rdfs:comment "A scalar value equal to the number of ancestor blocks. The genesis block has a number of zero."@en ;
	rdfs:label "Block number"@en ;
	ns:term_status "unstable" .
# 
# http://ethon.consensys.net/receiptsRoot

:receiptsRoot a owl:DatatypeProperty ;
	rdfs:subPropertyOf :MessageDataProperty ;
	a owl:FunctionalProperty ;
	rdfs:domain :ReceiptsTrie ;
	rdfs:range xsd:hexBinary ;
	:suggestedStringRepresentation "blockReceiptsRoot" ;
	rdfs:comment "The Keccak 256-bit hash of the root node of the trie structure populated with the receipts of each transaction in the transactions list portion of the block."@en ;
	rdfs:label "Receipts root"@en ;
	ns:term_status "unstable" .
# 
# http://ethon.consensys.net/stateRoot

:stateRoot a owl:DatatypeProperty ;
	rdfs:subPropertyOf :StateDataProperty ;
	a owl:FunctionalProperty ;
	rdfs:domain :State ;
	rdfs:range xsd:hexBinary ;
	:suggestedStringRepresentation "stateRoot" ;
	rdfs:comment "The Keccak 256-bit hash of the root node of the state trie that represents this state."@en ;
	rdfs:label "State root"@en ;
	ns:term_status "unstable" .
# 
# http://ethon.consensys.net/storageRoot

:storageRoot a owl:DatatypeProperty ;
	rdfs:subPropertyOf :AccountDataProperty ;
	a owl:FunctionalProperty ;
	rdfs:domain :AccountStorage ;
	rdfs:range xsd:hexBinary ;
	:suggestedStringRepresentation "storageRoot" ;
	rdfs:comment "A 256-bit hash of the root node of a Merkle Patricia tree that encodes the storage contents of the account (a mapping between 265-bit integer values), encoded into the trie as a mapping from the Keccak 256-bit hash of the 256-bit integer keys to the RLP-encoded 256-bit integer values."@en ;
	rdfs:label "Storage root"@en ;
	ns:term_status "unstable" .
# 
# http://ethon.consensys.net/transactionsRoot

:transactionsRoot a owl:DatatypeProperty ;
	rdfs:subPropertyOf :MessageDataProperty ;
	a owl:FunctionalProperty ;
	rdfs:domain :TxTrie ;
	rdfs:range xsd:hexBinary ;
	:suggestedStringRepresentation "blockTransactionsRoot" ;
	rdfs:comment "The Keccak 256-bit hash of the root node of the trie structure populated with each transaction in the transactions list portion of the block."@en ;
	rdfs:label "Transactions root"@en ;
	ns:term_status "unstable" .
# 
# http://ethon.consensys.net/txGasPrice

:txGasPrice a owl:DatatypeProperty ;
	rdfs:subPropertyOf :MessageDataProperty ;
	rdfs:domain :Tx ;
	rdfs:range xsd:integer ;
	:suggestedStringRepresentation "txGasPrice" ;
	rdfs:comment "Price in Wei to be paid per unit of gas for all computation costs incurred as a result of the execution of this transaction. This implies that contract messages resulting from the transaction pay the same gas price."@en ;
	rdfs:label "Transaction gas price"@en ;
	ns:term_status "unstable" .
# 
# http://ethon.consensys.net/txGasUsed

:txGasUsed a owl:DatatypeProperty ;
	rdfs:subPropertyOf :MessageDataProperty ;
	a owl:FunctionalProperty ;
	rdfs:domain :Tx ;
	rdfs:range xsd:integer ;
	:suggestedStringRepresentation "txGasUsed" ;
	rdfs:comment "The total amount of gas that was used for processing this Tx and all contract messages resulting from it. It is the sum of all msgGasUsed by this Tx and resulting contract messages."@en ;
	rdfs:label "Tx gas used"@en ;
	ns:term_status "unstable" .
# 
# http://ethon.consensys.net/txHash

:txHash a owl:DatatypeProperty ;
	rdfs:subPropertyOf :MessageDataProperty ;
	rdfs:domain :Tx ;
	rdfs:range xsd:hexBinary ;
	:suggestedStringRepresentation "txHash" ;
	rdfs:comment "The Keccak 256-bit hash of the transaction"@en ;
	rdfs:label "Tx hash"@en ;
	ns:term_status "unstable" .
# 
# http://ethon.consensys.net/txIndex

:txIndex a owl:DatatypeProperty ;
	rdfs:subPropertyOf :MessageDataProperty ;
	rdfs:domain :Tx ;
	rdfs:range xsd:integer ;
	:suggestedStringRepresentation "txIndex" ;
	rdfs:comment "The position of a transaction in a block."@en ;
	rdfs:label "Transaction index"@en ;
	ns:term_status "unstable" .
# 
# http://ethon.consensys.net/txLogsBloom

:txLogsBloom a owl:DatatypeProperty ;
	rdfs:subPropertyOf :MessageDataProperty ;
	rdfs:domain :Tx ;
	rdfs:range xsd:hexBinary ;
	:suggestedStringRepresentation "txLogsBloom" ;
	rdfs:comment """The bloom filter of log entries resulting from a transaction.

For a more detailed description of log filters in Ethereum, see [block blogs bloom filter](http://ethon.consensys.net/blockLogsBloom)."""@en ;
	rdfs:label "transaction logs bloom filter"@en ;
	rdfs:seeAlso :blockLogsBloom ;
	ns:term_status "unstable" .
# 
# http://ethon.consensys.net/txNonce

:txNonce a owl:DatatypeProperty ;
	rdfs:subPropertyOf :MessageDataProperty ;
	rdfs:domain :Tx ;
	rdfs:range xsd:integer ;
	:suggestedStringRepresentation "txNonce" ;
	rdfs:comment "A scalar value equal to the number of transactions sent by the sender."@en ;
	rdfs:label "Transaction nonce"@en ;
	ns:term_status "unstable" .
# 
# http://ethon.consensys.net/txR

:txR a owl:DatatypeProperty ;
	rdfs:subPropertyOf :MessageDataProperty ;
	rdfs:domain :Tx ;
	rdfs:range xsd:hexBinary ;
	:suggestedStringRepresentation "txR" ;
	rdfs:comment "The values txV, txR and txS correspond to the signature of the transaction and are used to determine the sender of the transaction. The txR value is a Byte array of length 32."@en ;
	rdfs:label "Transaction r-value"@en ;
	ns:term_status "unstable" .
# 
# http://ethon.consensys.net/txS

:txS a owl:DatatypeProperty ;
	rdfs:subPropertyOf :MessageDataProperty ;
	rdfs:domain :Tx ;
	rdfs:range xsd:hexBinary ;
	:suggestedStringRepresentation "txS" ;
	rdfs:comment "The values txV, txR and txS correspond to the signature of the transaction and are used to determine the sender of the transaction. The value txS is a byte array of length 32."@en ;
	rdfs:label "Transaction s-value"@en ;
	ns:term_status "unstable" .
# 
# http://ethon.consensys.net/txStatus

:txStatus a owl:DatatypeProperty ;
	rdfs:subPropertyOf :MessageDataProperty ;
	rdfs:domain :Tx ;
	rdfs:range xsd:boolean ;
	:suggestedStringRepresentation "txStatus" ;
	rdfs:comment "A status code for the transaction. False indicates failure (due to any operation that can cause the transaction or top-level call to revert) and true indicates success. This property was introduced with the Byzantium hard fork (EIP-658)."@en ;
	rdfs:label "Transaction status"@en ;
	ns:term_status "unstable" .
# 
# http://ethon.consensys.net/txV

:txV a owl:DatatypeProperty ;
	rdfs:subPropertyOf :MessageDataProperty ;
	rdfs:domain :Tx ;
	rdfs:range xsd:byte ;
	:suggestedStringRepresentation "txV" ;
	rdfs:comment "The values txV, txR and txS correspond to the signature of the transaction and are used to determine the sender of the transaction. The value txV specifies the sign and finiteness of the curve point. Since EIP-155 it is used to realize a replay attack protection. It is calculated in the following way: txV = CHAIN_ID * 2 + 36"@en ;
	rdfs:label "Transaction v-value"@en ;
	rdfs:seeAlso <https://github.com/ethereum/EIPs/issues/155> ;
	ns:term_status "unstable" .
# 
# http://ethon.consensys.net/uncleBeneficiaryReward

:uncleBeneficiaryReward a owl:DatatypeProperty ;
	rdfs:subPropertyOf :BlockDataProperty ;
	a owl:FunctionalProperty ;
	rdfs:domain :Uncle ;
	rdfs:range xsd:integer ;
	:suggestedStringRepresentation "uncleBenficiaryReward" ;
	rdfs:comment "The reward the beneficiary of an uncle receives if a block includes it. The reward amount depends how far up the Uncle is in the blockchain (the number of the block in which it is included minus the uncle's number). An uncle reward is only paid if the distance is smaller than 8. For a distance of 1 the reward is 7/8 of the block reward, for a distance of 7 the reward is 1/8 of the block reward."@en ;
	rdfs:label "Uncle beneficiary reward"@en ;
	ns:term_status "unstable" .
# 
# http://ethon.consensys.net/uncleIndex

:uncleIndex a owl:DatatypeProperty ;
	rdfs:subPropertyOf :BlockDataProperty ;
	rdfs:domain :Uncle ;
	rdfs:range xsd:integer ;
	:suggestedStringRepresentation "uncleIndex" ;
	rdfs:comment "Represents the order of uncles included in a block."@en ;
	rdfs:label "Uncle index"@en ;
	ns:term_status "unstable" .
# 
# http://ethon.consensys.net/value

:value a owl:DatatypeProperty ;
	rdfs:subPropertyOf :MessageDataProperty ;
	a owl:FunctionalProperty ;
	rdfs:domain :Msg ;
	rdfs:range xsd:integer ;
	:suggestedStringRepresentation "value" ;
	rdfs:comment "A scalar value equal to the number of Wei to be transferred to the Message call's recipient. In the case of contract creation it is the initial balance of the contract account, paid by the sending account."@en ;
	rdfs:label "value in Wei"@en ;
	ns:term_status "unstable" .
# 
# 
# 
# #################################################################
# #
# #    Classes
# #
# #################################################################
# 
# 
# http://ethon.consensys.net/Account

:Account a owl:Class ;
	rdfs:subClassOf :AccountConcept , _:genid18 .

_:genid18 a owl:Restriction ;
	owl:onProperty :hasState ;
	owl:someValuesFrom :AccountState .

:Account rdfs:subClassOf _:genid19 .

_:genid19 a owl:Restriction ;
	owl:onProperty :address ;
	owl:qualifiedCardinality "1"^^xsd:nonNegativeInteger ;
	owl:onDataRange xsd:hexBinary .

:Account owl:hasKey _:genid20 .

_:genid20 a rdf:List ;
	rdf:first :address ;
	rdf:rest rdf:nil .

:Account :simpleDefinition "There are two main types of accounts: external accounts (often referred to as \"wallet\" or simply \"account\") and contract accounts (usually just called \"contract\" or \"smart contract\"). An external account is what you need to use Ethereum. It is usually protected by a password. If you have the password you can send Ether from your account to another or use a contract. It has an Ethereum address (0x...) by which it is identified." ;
	:suggestedStringRepresentation "Account"@en ;
	rdfs:comment "*Account* is the superclass of all account types in Ethereum. All accounts are identified by an address (which, however, is derived differently for external and contract accounts) and an account state that contains the contract's balance and total message count, which is called its nonce. Contract accounts also have an associated storage state and EVM code. The address of an external account is derived from the public key of a public and private keypair, while a contract account address is a concatenation of the creator account's address and its nonce. Both contract accounts and external accounts can also be of type *protocol account* if they are specified in the Ethereum blockchain, i.e. the accounts pre-funded by the Ethereum crowdsale."@en ;
	rdfs:label "Account"@en ;
	ns:term_status "unstable" .
# 
# http://ethon.consensys.net/AccountConcept

:AccountConcept a owl:Class ;
	rdfs:subClassOf :EthOnConcept ;
	:suggestedStringRepresentation "AccountConcept"@en ;
	rdfs:comment "The group of all EthOn classes related to accounts."@en ;
	rdfs:label "EthOn Account concept"@en ;
	ns:term_status "unstable" .
# 
# http://ethon.consensys.net/AccountState

:AccountState a owl:Class ;
	rdfs:subClassOf :AccountConcept , :State ;
	:suggestedStringRepresentation "AccountState"@en ;
	rdfs:comment "State of an Ethereum account. It is comprised on four pieces of information: nonce, balance, storage root and code hash. The data is stored in a Merkle Patricia tree as a mapping between addresses and account states. The account state is part of the world state, as it resembles the state of exactly one account."@en ;
	rdfs:label "Account State"@en ;
	ns:term_status "unstable" .
# 
# http://ethon.consensys.net/AccountStorage

:AccountStorage a owl:Class ;
	rdfs:subClassOf :AccountConcept , :ModifiedMerklePatriciaTree ;
	:simpleDefinition "A data structure which contains the current storage state of a smart contract, i.e. the total supply of an ERC20 token and the mapping of account addresses to current balances." ;
	:suggestedStringRepresentation "AccountStorage"@en ;
	rdfs:comment "The account storage is part of the account state and it contains contains the values of all variables defined in the contract's code at a certain point in time. Usually Ethereum clients implement this structure as a Merkle Patricia Tree. Whenever any of the contract's variables are changed a new state is created."@en ;
	rdfs:label "Storage"@en ;
	ns:term_status "unstable" .
# 
# http://ethon.consensys.net/Block

:Block a owl:Class ;
	rdfs:subClassOf :BlockConcept , :StateTransition ;
	owl:hasKey _:genid21 .

_:genid21 a rdf:List ;
	rdf:first :blockHash ;
	rdf:rest rdf:nil .

:Block :simpleDefinition "A block is an entry in a blockchain. It contains a series of transactions as well as a cryptographic hash linking it to the previous block in the chain." ;
	:suggestedStringRepresentation "Block"@en ;
	rdfs:comment "A block is the basic element of a 'blockchain'. It functions as an entry in a distributed ledger, recording a series of transactions together with a reference to the previous block. A block is chained to its preceeding block by a cryptographic hash of its contents as a means of reference. Blocks contain an identifier for the final state after all transactions contained in it are validated. There is a consensus mechanism that provides incentives for nodes adding new blocks to the chain (\"miners\" in the Proof of Work protocol used by the main Ethereum network) that comply with the rules of Ethereum by issuing newly generated tokens ('Ether') to an account specified by the block's author."@en ;
	rdfs:label "Block"@en ;
	ns:term_status "unstable" .
# 
# http://ethon.consensys.net/BlockConcept

:BlockConcept a owl:Class ;
	rdfs:subClassOf :EthOnConcept ;
	:suggestedStringRepresentation "BlockConcept"@en ;
	rdfs:comment "The group of all EthOn classes related to blocks."@en ;
	rdfs:label "EthOn Block concept"@en ;
	ns:term_status "unstable" .
# 
# http://ethon.consensys.net/Blockchain

:Blockchain a owl:Class ;
	rdfs:subClassOf :NetworkConcept ;
	:suggestedStringRepresentation "Blockchain" ;
	rdfs:comment "An Ethereum blockchain is a distributed database that maintains a continuously-growing list of records called *blocks* secured from tampering and revision. Each block contains a timestamp and a link to a previous block in a Merkle tree structure."@en ;
	rdfs:label "Ethereum Blockchain"@en ;
	ns:term_status "unstable" .
# 
# http://ethon.consensys.net/CallContractMsg

:CallContractMsg a owl:Class ;
	rdfs:subClassOf :ContractMsg , _:genid22 .

_:genid22 a owl:Restriction ;
	owl:onProperty :to ;
	owl:qualifiedCardinality "1"^^xsd:nonNegativeInteger ;
	owl:onClass :ContractAccount .

:CallContractMsg :suggestedStringRepresentation "CallContractMsg" ;
	rdfs:comment "A call contract message is a contract message that calls a function in another contract."@en ;
	rdfs:label "Call Contract Message"@en ;
	ns:term_status "unstable" .
# 
# http://ethon.consensys.net/CallTx

:CallTx a owl:Class ;
	rdfs:subClassOf :Tx , _:genid23 .

_:genid23 a owl:Restriction ;
	owl:onProperty :to ;
	owl:qualifiedCardinality "1"^^xsd:nonNegativeInteger ;
	owl:onClass :ContractAccount .

:CallTx :suggestedStringRepresentation "CallTx" ;
	rdfs:comment "A type of transaction that is directed towards a contract account and calls a method in the contract's code."@en ;
	rdfs:label "Call Transaction"@en ;
	ns:term_status "unstable" .
# 
# http://ethon.consensys.net/ContractAccount

:ContractAccount a owl:Class ;
	rdfs:subClassOf :Account ;
	owl:disjointWith :ExternalAccount ;
	:simpleDefinition "A type of Ethereum account that represents a smart contract. Its behaviour is controlled by the logic in the smart contract's code. Like external accounts it is identified by an address." ;
	:suggestedStringRepresentation "ContractAccount"@en ;
	rdfs:comment "One of the two main types of accounts on Ethereum, a contract account is an account whose behaviour is controlled by a smart contract. Contract accounts are identified by their address which is derived from the creator account's address and nonce. A contract account has a non-empty associated EVM code. It's state data consists of the bytecode, the contract's balance and the storage state of the contract's code (for example the value of variables). A contract account can only act when it is triggered by a message. It may not create and sign transactions, but it can receive transactions from external accounts as well as send and receive contract messages, which may involve a transfer of Ether. Contract accounts can also contain events which create log entries when triggered."@en ;
	rdfs:label "Contract Account"@en ;
	ns:term_status "unstable" .
# 
# http://ethon.consensys.net/ContractMsg

:ContractMsg a owl:Class ;
	rdfs:subClassOf :Msg , _:genid24 .

_:genid24 a owl:Restriction ;
	owl:onProperty :from ;
	owl:qualifiedCardinality "1"^^xsd:nonNegativeInteger ;
	owl:onClass :ContractAccount .

:ContractMsg :suggestedStringRepresentation "ContractMsg" ;
	rdfs:comment "A contract message is passed between a contract account and any other account (external or contract). It is the result of an execution chain originally triggered by an external eccount."@en ;
	rdfs:label "Contract Message"@en ;
	ns:term_status "unstable" .
# 
# http://ethon.consensys.net/CreateContractMsg

:CreateContractMsg a owl:Class ;
	rdfs:subClassOf :ContractMsg , _:genid25 .

_:genid25 a owl:Restriction ;
	owl:onProperty :creates ;
	owl:qualifiedCardinality "1"^^xsd:nonNegativeInteger ;
	owl:onClass :ContractAccount .

:CreateContractMsg :suggestedStringRepresentation "CreateContractMsg" ;
	rdfs:comment "A create contract message is a subtype of a contract message that results in creation of a new contract account."@en ;
	rdfs:label "Create Contract Message"@en ;
	ns:term_status "unstable" .
# 
# http://ethon.consensys.net/CreateTx

:CreateTx a owl:Class ;
	rdfs:subClassOf :Tx , _:genid26 .

_:genid26 a owl:Restriction ;
	owl:onProperty :creates ;
	owl:qualifiedCardinality "1"^^xsd:nonNegativeInteger ;
	owl:onClass :ContractAccount .

:CreateTx :suggestedStringRepresentation "CreateTx" ;
	rdfs:comment "A type of transaction that results in creation of a new contract account."@en ;
	rdfs:label "Create Transaction"@en ;
	ns:term_status "unstable" .
# 
# http://ethon.consensys.net/EthOnConcept

:EthOnConcept a owl:Class ;
	:suggestedStringRepresentation "EthonConcept"@en ;
	rdfs:comment "Groups all classes and subclasses that are original to the EthOn OWL ontology."@en ;
	rdfs:label "EthOn Concept"@en ;
	ns:term_status "unstable" .
# 
# http://ethon.consensys.net/ExternalAccount

:ExternalAccount a owl:Class ;
	rdfs:subClassOf :Account ;
	:simpleDefinition "An Ethereum account usually controlled by a person. It is identified by an address (0x...) and a public/private key-pair." ;
	:suggestedStringRepresentation "ExternalAccount"@en ;
	rdfs:comment "One of the two main types of accounts on Ethereum, an external account is an account controlled by an external actor (as opposed to a contract account). The unique identifier of an external account is its address. It consists of the rightmost 160 bits of the keccak 256 hash of its public key (example: 0x1a1138875dAB9E0AC8b0fd4a37EEAC5eb26B870B). There is only one way external accounts can actively change the state of the blockchain. They can be used to send a valid transaction to the Ethereum blockchain. The transaction can be directed towards other external accounts or towards contract accounts. Since the private key is needed for sending, a valid transaction can only be created by the person or entity controlling the private key of the external account. Besides being target of transactions, external accounts can also be the target of contract messages, block beneficiary rewards, uncle beneficiary rewards or payouts of contract accounts that have self-destructed."@en ;
	rdfs:label "Externally Controlled Account"@en ;
	ns:term_status "unstable" .
# 
# http://ethon.consensys.net/ExternalActor

:ExternalActor a owl:Class ;
	rdfs:subClassOf :AccountConcept , <http://xmlns.com/foaf/0.1/Agent> ;
	:simpleDefinition "A person or other entity controlling one or more external accounts, which can interact with Ethereum by signing transactions with a public-private keypair." ;
	:suggestedStringRepresentation "ExternalActor"@en ;
	rdfs:comment "A person or other entity able to interface with an Ethereum node. An external actor controls the private-public keypair of one or more external accounts. It can change the state of the blockchain by sending signed and valid transactions. Without using a keypair, external actors can also inspect and read from the blockchain and its state."@en ;
	rdfs:label "External Actor"@en ;
	ns:term_status "unstable" .
# 
# http://ethon.consensys.net/FullNode

:FullNode a owl:Class ;
	rdfs:subClassOf :Node ;
	owl:disjointWith :LightNode ;
	:simpleDefinition "A piece of software which connects fully to an Ethereum network, storing its complete history and having the ability to submit new blocks to the blockchain (i.e. through mining)." ;
	:suggestedStringRepresentation "FullNode" ;
	rdfs:comment "A full node is a participant in an Ethereum network that keeps a record of the full blockchain, the full state and may engage in mining."@en ;
	rdfs:label "Ethereum Full Node"@en ;
	ns:term_status "unstable" .
# 
# http://ethon.consensys.net/GenesisBlock

:GenesisBlock a owl:Class ;
	rdfs:subClassOf :Block ;
	:suggestedStringRepresentation "GenesisBlock" ;
	rdfs:comment "A genesis block is the unmined, deliberately created, very first block in a blockchain. It has no predecessors, i.e. no parent block."@en ;
	rdfs:label "Genesis Block"@en ;
	ns:term_status "unstable" .
# 
# http://ethon.consensys.net/LightNode

:LightNode a owl:Class ;
	rdfs:subClassOf :Node ;
	:simpleDefinition "A piece of software which connects to an Ethereum network in a limited capacity, i.e. a smart phone wallet app which neither mines nor downloads the full blockchain, but can still send and receive messages." ;
	:suggestedStringRepresentation "LightNode" ;
	rdfs:comment "A light node is a participant in an Ethereum network that does not completely do any of the following: store the complete blockchain, store the complete world state, engage in mining."@en ;
	rdfs:label "Ethereum Light Node"@en ;
	ns:term_status "unstable" .
# 
# http://ethon.consensys.net/LogEntry

:LogEntry a owl:Class ;
	rdfs:subClassOf :MessageConcept ;
	:suggestedStringRepresentation "LogEntry" ;
	rdfs:comment "A log entry is the result of an event in a smart contract, emitted during creation or execution of a contract account's code. It is related to the Tx it was created in, the contract account that had the event, a series of 32-bytes log topics and a number of bytes of data."@en ;
	rdfs:label "Log Entry"@en ;
	ns:term_status "unstable" .
# 
# http://ethon.consensys.net/LogTopic

:LogTopic a owl:Class ;
	rdfs:subClassOf :MessageConcept ;
	:suggestedStringRepresentation "LogTopic" ;
	rdfs:comment "A 32-bytes long topic of a log entry. The log topics of a log entry have an order given by a topic index value."@en ;
	rdfs:label "Log Topic"@en ;
	ns:term_status "unstable" .
# 
# http://ethon.consensys.net/MessageConcept

:MessageConcept a owl:Class ;
	rdfs:subClassOf :EthOnConcept ;
	rdfs:comment "The group of all EthOn classes related to messages."@en ;
	rdfs:label "EthOn Message concept"@en ;
	ns:term_status "unstable" .
# 
# http://ethon.consensys.net/ModifiedMerklePatriciaTree

:ModifiedMerklePatriciaTree a owl:Class ;
	rdfs:subClassOf :EthOnConcept ;
	:suggestedStringRepresentation "ModifiedMerklePatriciaTree"@en ;
	rdfs:comment "Merkle Patricia trees provide a cryptographically authenticated data structure that can be used to store all (key, value) bindings, although for the scope of this paper we are restricting keys and values to strings (to remove this restriction, just use any serialization format for other data types). They are fully deterministic, meaning that a Patricia tree with the same (key,value) bindings is guaranteed to be exactly the same down to the last byte and therefore have the same root hash, provide the holy grail of O(log(n)) efficiency for inserts, lookups and deletes, and are much easier to understand and code than more complex comparison-based alternatives like red-black trees."@en ;
	rdfs:label "Merkle Patricia Tree"@en ;
	rdfs:seeAlso <https://github.com/ethereum/wiki/wiki/Patricia-Tree> ;
	ns:term_status "unstable" .
# 
# http://ethon.consensys.net/Msg

:Msg a owl:Class ;
	rdfs:subClassOf :MessageConcept , :StateTransition ;
	:suggestedStringRepresentation "Msg" ;
	rdfs:comment "Data (as a set of bytes) and value (specified as Ether) that is passed between two accounts, either through the deterministic operation of an autonomous object (contract account) or the cryptographically secure signature of an external account."@en ;
	rdfs:label "Message"@en ;
	ns:term_status "unstable" .
# 
# http://ethon.consensys.net/Network

:Network a owl:Class ;
	rdfs:subClassOf :NetworkConcept ;
	:suggestedStringRepresentation "Network" ;
	rdfs:comment "An Ethereum network is the group of all nodes that conform to a certain protocol variant."@en ;
	rdfs:label "Ethereum Network"@en ;
	ns:term_status "unstable" .
# 
# http://ethon.consensys.net/NetworkConcept

:NetworkConcept a owl:Class ;
	rdfs:subClassOf :EthOnConcept ;
	:suggestedStringRepresentation "NetworkConcept" ;
	rdfs:comment "The group of all EthOn classes related to networks."@en ;
	rdfs:label "EthOn Network Concept."@en .
# 
# http://ethon.consensys.net/Node

:Node a owl:Class ;
	rdfs:subClassOf :NetworkConcept ;
	:simpleDefinition "A piece of software participating in the Ethereum network." ;
	:suggestedStringRepresentation "Node" ;
	rdfs:comment "A participant in an Ethereum network, specifically an instance of one of the client implementations, which may be either a full node or a light node."@en ;
	rdfs:label "Node"@en ;
	ns:term_status "unstable" .
# 
# http://ethon.consensys.net/PostBlockState

:PostBlockState a owl:Class ;
	rdfs:subClassOf :PostTxState .
# 
# http://ethon.consensys.net/PostMsgState

:PostMsgState a owl:Class ;
	rdfs:subClassOf :WorldState .
# 
# http://ethon.consensys.net/PostTxState

:PostTxState a owl:Class ;
	rdfs:subClassOf :PostMsgState .
# 
# http://ethon.consensys.net/ProtocolAccount

:ProtocolAccount a owl:Class ;
	rdfs:subClassOf :Account ;
	:simpleDefinition "An account that was created together with the blockchain itself or during a protcol update and can have an initial balance, e.g. from the crowdfunding of the blockchain." ;
	:suggestedStringRepresentation "PrefundedAccount"@en ;
	rdfs:comment "A protocol account is a type of account in Ethereum. Protocol accounts are specified in the Ethereum protocol, and have so far only been used to store the initial balance for users who participated in the Ethereum crowdsale. Protocol accounts could be added with any protocol change and may be either external accounts or contract accounts."@en ;
	rdfs:label "Protocol Account"@en ;
	ns:term_status "unstable" .
# 
# http://ethon.consensys.net/ProtocolState

:ProtocolState a owl:Class ;
	rdfs:subClassOf :AccountState ;
	:suggestedStringRepresentation "ProtocolState"@en ;
	rdfs:comment "This is a special state that can be created after specification of the protocol or any protocol change. It allows for setting balances of accounts, e.g. for prefunded accounts, creating predefined contract accounts with storage or setting any other state property as part of the protocol specification."@en ;
	rdfs:label "ProtocolState"@en ;
	ns:term_status "unstable" .
# 
# http://ethon.consensys.net/ProtocolVariant

:ProtocolVariant a owl:Class ;
	rdfs:subClassOf :NetworkConcept ;
	:suggestedStringRepresentation "EthereumProtocolVariant" ;
	rdfs:comment "A variant of the Ethereum protocol. Changes in the protocol result in a fork."@en ;
	rdfs:label "Ethereum Protocol Variant"@en ;
	rdfs:seeAlso <https://ethereum.stackexchange.com/questions/13014/please-confirm-what-the-hard-forks-of-ethereum-were-and-when-they-took-place> ;
	ns:term_status "unstable" .
# 
# http://ethon.consensys.net/ReceiptsTrie

:ReceiptsTrie a owl:Class ;
	rdfs:subClassOf :BlockConcept , :MessageConcept , :ModifiedMerklePatriciaTree ;
	:suggestedStringRepresentation "ReceiptsTrie" ;
	rdfs:comment "A trie structure that stores transaction receipts. Each block has a reference to the root hash of a receipts trie that stores the receipts of the transactions included in the block."@en ;
	rdfs:label "Receipts Trie"@en ;
	ns:term_status "unstable" .
# 
# http://ethon.consensys.net/SelfdestructContractMsg

:SelfdestructContractMsg a owl:Class ;
	rdfs:subClassOf :ContractMsg ;
	:suggestedStringRepresentation "SelfdestructContractMsg" ;
	rdfs:comment "A selfdestruct contract message is a contract message that deletes the originating contract and refunds its balance to the receiver of the message."@en ;
	rdfs:label "Selfdestruct Contract Message"@en ;
	rdfs:seeAlso <https://github.com/ethereum/EIPs/blob/master/EIPS/eip-6.md> ;
	ns:term_status "unstable" .
# 
# http://ethon.consensys.net/State

:State a owl:Class ;
	rdfs:subClassOf :StateConcept ;
	owl:disjointWith :StateTransition ;
	:suggestedStringRepresentation "State" ;
	rdfs:comment "The concept of a state in a generic state transition system."@en ;
	rdfs:label "State"@en ;
	rdfs:seeAlso <https://en.wikipedia.org/wiki/Transition_system> , <https://en.wikipedia.org/wiki/State_(computer_science)> ;
	ns:term_status "unstable" .
# 
# http://ethon.consensys.net/StateConcept

:StateConcept a owl:Class ;
	rdfs:subClassOf :EthOnConcept ;
	rdfs:comment "The group of all EthOn classes related to state."@en ;
	rdfs:label "EthOn State Concept"@en ;
	ns:term_status "unstable" .
# 
# http://ethon.consensys.net/StateTransition

:StateTransition a owl:Class ;
	rdfs:subClassOf :StateConcept ;
	:suggestedStringRepresentation "StateTransition" ;
	rdfs:comment "The concept of a transition in a state transition system."@en ;
	rdfs:label "State Transition"@en ;
	rdfs:seeAlso <https://en.wikipedia.org/wiki/Transition_system> ;
	ns:term_status "unstable" .
# 
# http://ethon.consensys.net/Tx

:Tx a owl:Class ;
	rdfs:subClassOf :Msg , _:genid27 .

_:genid27 a owl:Restriction ;
	owl:onProperty :from ;
	owl:qualifiedCardinality "1"^^xsd:nonNegativeInteger ;
	owl:onClass :ExternalAccount .

:Tx :suggestedStringRepresentation "Tx" ;
	rdfs:comment "Transactions are messages between two accounts that may transfer Ether and may contain a payload. Transactions always originate from an external account that is controlled by an external actor by means of a private key.  The execution of a transaction creates a 'transaction receipt'."@en ;
	rdfs:label "Transaction"@en ;
	ns:term_status "unstable" .
# 
# http://ethon.consensys.net/TxReceipt

:TxReceipt a owl:Class ;
	rdfs:subClassOf :MessageConcept ;
	:suggestedStringRepresentation "TxReceipt" ;
	rdfs:comment "The transaction receipt is comprised of the post-transaction-state, the cumulative gas used in the block containing the transaction receipt as of immediately after the transaction has happened, the set of logs created through execution of the transaction, the bloom filter composed from information in those logs and a boolean status code indicating success of failure of the transaction. However, in EthOn these properties are not related to the receipt but to the transaction directly, in order to simplify the resulting data model."@en ;
	rdfs:label "Transaction Receipt"@en ;
	ns:term_status "unstable" .
# 
# http://ethon.consensys.net/TxTrie

:TxTrie a owl:Class ;
	rdfs:subClassOf :BlockConcept , :MessageConcept , :ModifiedMerklePatriciaTree ;
	:suggestedStringRepresentation "TxTrie" ;
	rdfs:comment "A trie structure that stores transactions. The header of a block contains a reference to the root of a Tx trie with all transactions contained in the block."@en ;
	rdfs:label "Transactions Trie"@en ;
	ns:term_status "unstable" .
# 
# http://ethon.consensys.net/Uncle

:Uncle a owl:Class ;
	rdfs:subClassOf :Block ;
	:suggestedStringRepresentation "Uncle"@en ;
	rdfs:comment "An uncle is the direct child of the k'th generation ancestor of a block B, where 2<=k<=7 but not a direct ancestor of B. Uncles are blockchain blocks found by a miner, when a different miner has already found another block for the corresponding place in the blockchain. They are also known as “stale blocks”. The parent of an uncle is an ancestor of the inserting block, located at the tip of the blockchain."@en ;
	rdfs:label "Uncle"@en ;
	ns:term_status "unstable" .
# 
# http://ethon.consensys.net/ValueContractMsg

:ValueContractMsg a owl:Class ;
	rdfs:subClassOf :ContractMsg , _:genid28 .

_:genid28 a owl:Restriction ;
	owl:onProperty :to ;
	owl:qualifiedCardinality "1"^^xsd:nonNegativeInteger ;
	owl:onClass :Account .

:ValueContractMsg :suggestedStringRepresentation "ValueContractMsg" ;
	rdfs:comment "A Value Contract Message is a Contract Message that does not call a function in a smart contract and doesn't create a new smart contract. Even though it is called \"value\" Contract Message, it can have a value of 0 Ether. Value Contract Messages can have a payload as long as that payload doesn't trigger the execution of a function in a smart contract."@en ;
	rdfs:label "Value Contract Message"@en ;
	ns:term_status "unstable" .
# 
# http://ethon.consensys.net/ValueTx

:ValueTx a owl:Class ;
	rdfs:subClassOf :Tx , _:genid29 .

_:genid29 a owl:Restriction ;
	owl:onProperty :to ;
	owl:qualifiedCardinality "1"^^xsd:nonNegativeInteger ;
	owl:onClass :Account .

:ValueTx :suggestedStringRepresentation "ValueTx" ;
	rdfs:comment "A Value Transaction is a Transaction that does not call a function in a smart contract and doesn't create a new smart contract. Even though it is called \"value\" Transaction, Transactions with a value of 0 Ether can be Value Transaction. Value Transactions can have a payload as long as that payload doesn't trigger the execution of a function in a smart contract."@en ;
	rdfs:label "Value Transaction"@en ;
	ns:term_status "unstable" .
# 
# http://ethon.consensys.net/WorldState

:WorldState a owl:Class ;
	rdfs:subClassOf :ModifiedMerklePatriciaTree , :State ;
	:suggestedStringRepresentation "State"@en ;
	rdfs:comment "The world state, is a mapping between addresses (160-bit identifiers) of all accounts and their states (a data structure serialised as Recursive Length Prefix). The mapping is not stored on the blockchain itself but in a modified Merkle Patricia tree. An individual state is identified by the root hash of the trie."@en ;
	rdfs:label "World State"@en ;
	ns:term_status "unstable" .
# 
# http://xmlns.com/foaf/0.1/Agent

<http://xmlns.com/foaf/0.1/Agent> a owl:Class ;
	rdfs:isDefinedBy <http://xmlns.com/foaf/0.1/> .
# 
# 
# 
# #################################################################
# #
# #    Individuals
# #
# #################################################################
# 
# 
# http://ethereum.ethstats.io/Block_0

<http://ethereum.ethstats.io/Block_0> a owl:NamedIndividual , :Block , :GenesisBlock ;
	:conformsTo :ProtocolVariant_Frontier ;
	:number "0"^^xsd:integer ;
	rdfs:label "Block 0"@en .
# 
# http://ethereum.ethstats.io/Block_1150000

<http://ethereum.ethstats.io/Block_1150000> a owl:NamedIndividual , :Block ;
	:conformsTo :ProtocolVariant_Homestead ;
	:number "1150000"^^xsd:integer ;
	rdfs:label "Block 1150000"@en .
# 
# http://ethereum.ethstats.io/Block_1920000

<http://ethereum.ethstats.io/Block_1920000> a owl:NamedIndividual , :Block ;
	:conformsTo :ProtocolVariant_DAO ;
	:number "1920000"^^xsd:integer ;
	rdfs:label "Block 1920000"@en .
# 
# http://ethereum.ethstats.io/Block_200000

<http://ethereum.ethstats.io/Block_200000> a owl:NamedIndividual , :Block ;
	:conformsTo :ProtocolVariant_IceAge ;
	:number "200000"^^xsd:integer ;
	rdfs:label "Block 200000"@en .
# 
# http://ethereum.ethstats.io/Block_2463000

<http://ethereum.ethstats.io/Block_2463000> a owl:NamedIndividual , :Block ;
	:conformsTo :ProtocolVariant_TangerineWhistle ;
	:number "2463000"^^xsd:integer ;
	rdfs:label "Block 2463000"@en .
# 
# http://ethereum.ethstats.io/Block_2675000

<http://ethereum.ethstats.io/Block_2675000> a owl:NamedIndividual , :Block ;
	:conformsTo :ProtocolVariant_SpuriousDragon ;
	:number "2675000"^^xsd:integer ;
	rdfs:label "Block 2675000"@en .
# 
# http://ethereum.ethstats.io/Block_4370000

<http://ethereum.ethstats.io/Block_4370000> a owl:NamedIndividual , :Block ;
	:conformsTo :ProtocolVariant_Byzantium ;
	:number "4370000"^^xsd:integer ;
	rdfs:label "Block 4370000"@en .
# 
# http://ethereum.ethstats.io/EthereumFoundationMainChain

<http://ethereum.ethstats.io/EthereumFoundationMainChain> a owl:NamedIndividual , :Blockchain ;
	:containsCanonicalBlock <http://ethereum.ethstats.io/Block_0> , <http://ethereum.ethstats.io/Block_1150000> , <http://ethereum.ethstats.io/Block_1920000> , <http://ethereum.ethstats.io/Block_200000> , <http://ethereum.ethstats.io/Block_2463000> , <http://ethereum.ethstats.io/Block_2675000> , <http://ethereum.ethstats.io/Block_4370000> ;
	rdfs:label "Ethereum Foundation main chain"@en ;
	rdfs:seeAlso <http://ethereum.ethstats.io/EthereumFoundationMainChain> .
# 
# http://ethon.consensys.net/ProtocolVariant_Byzantium

:ProtocolVariant_Byzantium a owl:NamedIndividual , :ProtocolVariant ;
	rdfs:comment "The Byzantium protocol change is the first step of a the Metropolis development phase. It adds two opcodes (`REVERT` and `STATICCALL`), adds a status field to transaction receipts, introduces precompiled contracts to allow zk-snarks and other cryptography, support for variable length return values, takes uncles into account when adjusting the difficulty and delays the difficulty bomb by 1 year."@en ;
	rdfs:label "Byzantium"@en ;
	rdfs:seeAlso <https://blog.ethereum.org/2017/10/12/byzantium-hf-announcement/> , <https://github.com/ethereum/EIPs/issues/100> , <https://github.com/ethereum/EIPs/pull/198> , <https://github.com/ethereum/EIPs/pull/206> , <https://github.com/ethereum/EIPs/pull/211> , <https://github.com/ethereum/EIPs/pull/212> , <https://github.com/ethereum/EIPs/pull/213> , <https://github.com/ethereum/EIPs/pull/214> , <https://github.com/ethereum/EIPs/pull/658> , <https://github.com/ethereum/EIPs/pull/669> .
# 
# http://ethon.consensys.net/ProtocolVariant_DAO

:ProtocolVariant_DAO a owl:NamedIndividual , :ProtocolVariant ;
	:hasHardFork :ProtocolVariant_TangerineWhistle ;
	rdfs:comment """The DAO protocol change was a hard fork intended to minimize the effects of the DAO heist. It allowed for all investments in the DAO to be payed back to the investers. This hard fork was highly contentious and the non-forked chain has proven to be long-lived (\"Ethereum Classic\").

As a result of this fork block 1920000 introduced an irregular state change to transfer ~12M ETH into a recovery contract."""@en ;
	rdfs:label "DAO"@en ;
	rdfs:seeAlso <https://blog.ethereum.org/2016/07/20/hard-fork-completed/> .
# 
# http://ethon.consensys.net/ProtocolVariant_Frontier

:ProtocolVariant_Frontier a owl:NamedIndividual , :ProtocolVariant ;
	:hasHardFork :ProtocolVariant_IceAge ;
	rdfs:comment "The original Ethereum protocol variant before any forks happened."@en ;
	rdfs:label "Frontier"@en ;
	rdfs:seeAlso <https://blog.ethereum.org/2015/07/22/frontier-is-coming-what-to-expect-and-how-to-prepare/> .
# 
# http://ethon.consensys.net/ProtocolVariant_Homestead

:ProtocolVariant_Homestead a owl:NamedIndividual , :ProtocolVariant ;
	:hasHardFork :ProtocolVariant_DAO ;
	rdfs:comment "The homestead protocol variant implemented EIP 2, 7 and 8. EIP 7 introduced a new Opcode `DELEGATECALL`."@en ;
	rdfs:label "Homestead"@en ;
	rdfs:seeAlso <https://blog.ethereum.org/2016/02/29/homestead-release/> , <https://github.com/ethereum/EIPs/blob/master/EIPS/eip-2.md> , <https://github.com/ethereum/EIPs/blob/master/EIPS/eip-606.md> , <https://github.com/ethereum/EIPs/blob/master/EIPS/eip-7.md> , <https://github.com/ethereum/EIPs/blob/master/EIPS/eip-8.md> .
# 
# http://ethon.consensys.net/ProtocolVariant_IceAge

:ProtocolVariant_IceAge a owl:NamedIndividual , :ProtocolVariant ;
	:hasHardFork :ProtocolVariant_Homestead ;
	rdfs:comment "The Ice Age protocol variant mainly introduced the \"difficulty bomb\"."@en ;
	rdfs:label "Ice Age"@en ;
	rdfs:seeAlso <https://blog.ethereum.org/2015/08/04/ethereum-protocol-update-1/> .
# 
# http://ethon.consensys.net/ProtocolVariant_SpuriousDragon

:ProtocolVariant_SpuriousDragon a owl:NamedIndividual , :ProtocolVariant ;
	:hasHardFork :ProtocolVariant_Byzantium ;
	rdfs:comment "The main purpose of the Spurious Dragon protocol variant was state clearing after the DOS attacks. It is the second hard fork that was done as a reaction to the DOS attacks that occured in September and October 2016. This protocol variant also includes some changes to opcode pricing and replay attack protection."@en ;
	rdfs:label "Spurious Dragon"@en ;
	rdfs:seeAlso <https://blog.ethereum.org/2016/11/18/hard-fork-no-4-spurious-dragon/> , <https://github.com/ethereum/EIPs/blob/master/EIPS/eip-155.md> , <https://github.com/ethereum/EIPs/blob/master/EIPS/eip-160.md> , <https://github.com/ethereum/EIPs/blob/master/EIPS/eip-161.md> , <https://github.com/ethereum/EIPs/blob/master/EIPS/eip-170.md> , <https://github.com/ethereum/EIPs/blob/master/EIPS/eip-606.md> .
# 
# http://ethon.consensys.net/ProtocolVariant_TangerineWhistle

:ProtocolVariant_TangerineWhistle a owl:NamedIndividual , :ProtocolVariant ;
	:hasHardFork :ProtocolVariant_SpuriousDragon ;
	rdfs:comment "The Tangerine Whistle protocol variant resulted in a hard fork that was the first of two steps to protect the Ethereum main chain from DOS attacks. These attacks happened in September and October 2016 and resulted in large delays for transaction processing. The changes maiinly affect the gas cost for IO-heavy operations."@en ;
	rdfs:label "Tangerine Whistle"@en ;
	rdfs:seeAlso <https://blog.ethereum.org/2016/10/18/faq-upcoming-ethereum-hard-fork/> , <https://github.com/ethereum/EIPs/blob/master/EIPS/eip-150.md> .
# 
# 
# 
# #################################################################
# #
# #    General axioms
# #
# #################################################################
# 
# 

_:genid30 a owl:AllDisjointClasses ;
	owl:members _:genid34 .

_:genid34 a rdf:List ;
	rdf:first :Block ;
	rdf:rest _:genid33 .

_:genid33 a rdf:List ;
	rdf:first :ReceiptsTrie ;
	rdf:rest _:genid32 .

_:genid32 a rdf:List ;
	rdf:first :TxTrie ;
	rdf:rest _:genid31 .

_:genid31 a rdf:List ;
	rdf:first :Uncle ;
	rdf:rest rdf:nil .
# 

_:genid35 a owl:AllDisjointClasses ;
	owl:members _:genid39 .

_:genid39 a rdf:List ;
	rdf:first :Blockchain ;
	rdf:rest _:genid38 .

_:genid38 a rdf:List ;
	rdf:first :Network ;
	rdf:rest _:genid37 .

_:genid37 a rdf:List ;
	rdf:first :Node ;
	rdf:rest _:genid36 .

_:genid36 a rdf:List ;
	rdf:first :ProtocolVariant ;
	rdf:rest rdf:nil .
# 

_:genid40 a owl:AllDisjointClasses ;
	owl:members _:genid43 .

_:genid43 a rdf:List ;
	rdf:first :CallContractMsg ;
	rdf:rest _:genid42 .

_:genid42 a rdf:List ;
	rdf:first :CreateContractMsg ;
	rdf:rest _:genid41 .

_:genid41 a rdf:List ;
	rdf:first :ValueContractMsg ;
	rdf:rest rdf:nil .
# 

_:genid44 a owl:AllDisjointClasses ;
	owl:members _:genid47 .

_:genid47 a rdf:List ;
	rdf:first :CallTx ;
	rdf:rest _:genid46 .

_:genid46 a rdf:List ;
	rdf:first :CreateTx ;
	rdf:rest _:genid45 .

_:genid45 a rdf:List ;
	rdf:first :ValueTx ;
	rdf:rest rdf:nil .
# 
# Generated by the OWL API (version 4.2.6.20160910-2108) https://github.com/owlcs/owlapi
